Add types for the rest of slices (where possible)

src/go_lang/slice.v
@@ -1,5 +1,5 @@
 From Perennial.go_lang Require Export lang notation.
-From Perennial.go_lang Require Import notation struct.
+From Perennial.go_lang Require Import struct typing.
 
 (** * Slice library
 
@@ -7,14 +7,27 @@ From Perennial.go_lang Require Import notation struct.
     soundly approximates slices as never having extra capacity.
  *)
 
+Open Scope heap_types.
+
 Module slice.
   Definition sliceS := mkStruct ["p"; "len"].
+  Definition T t := prodT (refT t) intT.
   Section fields.
     Context {ext:ext_op}.
     Definition ptr := structF! sliceS "p".
     Definition len: val := structF! sliceS "len".
+    Theorem ptr_t t Γ : Γ ⊢ ptr : (T t -> refT t).
+    Proof.
+      typecheck.
+    Qed.
+    Theorem len_t t Γ : Γ ⊢ len : (T t -> intT).
+    Proof.
+      typecheck.
+    Qed.
   End fields.
 End slice.
+
+Hint Resolve slice.ptr_t slice.len_t : types.
 
 (*
 Eval compute in get_field sliceS "p".
@@ -27,14 +40,24 @@ Section go_lang.
   Local Coercion Var' : string >-> expr.
 
 Definition NewByteSlice: val :=
-  λ: "sz",
+  λ: (annot "sz" intT),
   let: "p" := AllocN "sz" #(LitByte 0) in
   ("p", "sz").
 
+Theorem NewByteSlice_t Γ : Γ ⊢ NewByteSlice : (intT -> slice.T byteT).
+Proof.
+  typecheck.
+Qed.
+
 Definition MemCpy: val :=
-  λ: "dst" "src" "n",
+  λ: "dst" "src" (annot "n" intT),
     for: "i" < "n" :=
     ("dst" +ₗ "i") <- !("src" +ₗ "i").
+
+Theorem MemCpy_t Γ t : Γ ⊢ MemCpy : (refT t -> refT t -> intT -> unitT).
+Proof.
+  typecheck.
+Qed.
 
 (* explicitly recursive version of MemCpy *)
 Definition MemCpy_rec: val :=
@@ -44,8 +67,18 @@ Definition MemCpy_rec: val :=
     else "dst" <- !"src";;
          "memcpy" ("dst" +ₗ #1) ("src" +ₗ #1) ("n" - #1).
 
+Theorem MemCpy_rec_t Γ t : Γ ⊢ MemCpy_rec : (refT t -> refT t -> intT -> unitT).
+Proof.
+  typecheck.
+Qed.
+
 Definition SliceSkip: val :=
   λ: "s" "n", (slice.ptr "s" +ₗ "n", slice.len "s" - "n").
+
+Theorem SliceSkip_t Γ t : Γ ⊢ SliceSkip : (slice.T t -> intT -> slice.T t).
+Proof.
+  typecheck.
+Qed.
 
 Definition SliceTake: val :=
   λ: "s" "n", if: slice.len "s" < "n"
@@ -56,6 +89,11 @@ Definition SliceGet: val :=
   λ: "s" "i",
   !(slice.ptr "s" +ₗ "i").
 
+Theorem SliceGet_t Γ t : Γ ⊢ SliceGet : (slice.T t -> intT -> t).
+Proof.
+  typecheck.
+Qed.
+
 Definition SliceAppend: val :=
   λ: "s1" "s2",
   let: "p" := AllocN (slice.len "s1" + slice.len "s2") #() in
@@ -63,6 +101,12 @@ Definition SliceAppend: val :=
   MemCpy ("p" +ₗ slice.len "s2") (slice.ptr "s2");;
   (* TODO: unsound, need to de-allocate s1.p *)
   ("p", slice.len "s1" + slice.len "s2").
+
+(* doesn't work since initial value is of wrong type
+Theorem SliceAppend_t Γ t : Γ ⊢ SliceAppend : (slice.T t -> slice.T t -> slice.T t).
+Proof.
+  typecheck.
+Qed. *)
 
 Definition UInt64Put: val :=
   λ: "p" "n",
