src/go_lang/typing.v
@@ -10,8 +10,11 @@ Inductive ty :=
 | refT (t: ty)
 .
 
-Reserved Notation "Γ ⊢ e : A" (at level 91, e at next level, A at level 90).
-Reserved Notation "Γ '⊢v' v : A" (at level 91, v at next level, A at level 90).
+Infix "*" := prodT : heap_type.
+Infix "->" := arrowT : heap_type.
+
+Reserved Notation "Γ ⊢ e : A" (at level 74, e, A at next level).
+Reserved Notation "Γ '⊢v' v : A" (at level 74, v, A at next level).
 
 Definition Ctx := string -> option ty.
 Instance empty_ctx : Empty Ctx := fun _ => None.
@@ -112,7 +115,7 @@ Section go_lang.
   where "Γ ⊢v v : A" := (val_hasTy Γ v A)
   .
 
-  Theorem rec_expr_hasTy_eq Γ Γ' f x e t1 t2 :
+  Theorem rec_expr_hasTy_eq t1 t2 Γ Γ' f x e :
     Γ' = (<[f := arrowT t1 t2]> $ <[x := t1]> $ Γ) ->
     Γ' ⊢ e : t2 ->
     Γ ⊢ Rec f x e : arrowT t1 t2.
@@ -120,57 +123,44 @@ Section go_lang.
     intros; subst; econstructor; eauto.
   Qed.
 
+  Inductive type_annot :=
+  | annot (e:string) (t:ty).
+
+  Definition annot_e a := let 'annot e _  := a in e.
+
 End go_lang.
 
-Delimit Scope heap_types with T.
-Notation "Γ ⊢ e : A" := (expr_hasTy Γ e A) : heap_types.
-Notation "Γ ⊢v v : A" := (val_hasTy Γ v A) : heap_types.
-Notation "⊢ v : A" := (base_lit_hasTy v A) (at level 90, only printing) : heap_types.
-Notation "⊢ e : A" := (expr_hasTy ∅ e A) (at level 90, e at next level, A at next level) : heap_types.
+Notation "v :: t" := (annot v t) (only printing) : expr_scope.
+Coercion annot_e : type_annot >-> string.
 
-From Perennial.go_lang Require Import slice.
-Definition sliceT t : ty := prodT (refT t) intT.
+Delimit Scope heap_types with T.
+Delimit Scope heap_type with ht.
+Notation "Γ ⊢ e : A" := (expr_hasTy Γ%ht e A%ht) : heap_types.
+Notation "Γ ⊢v v : A" := (val_hasTy Γ%ht v A%ht) : heap_types.
+Notation "⊢ v : A" := (base_lit_hasTy v%V A%ht) (at level 90, only printing) : heap_types.
+Notation "⊢ e : A" := (expr_hasTy ∅ e%E A%ht) (at level 90, e at next level, A at next level) : heap_types.
 
 Theorem insert_anon t : (<[BAnon := t]> : Ctx -> Ctx) = (fun Γ => Γ).
 Proof.
   reflexivity.
 Qed.
 
-Local Ltac simp := unfold For; simpl; rewrite ?insert_anon.
-Local Ltac type_step :=
+Hint Constructors expr_hasTy : types.
+Hint Constructors val_hasTy : types.
+Hint Constructors base_lit_hasTy : types.
+
+Local Ltac simp := unfold For; cbv -[insert Z_to_byte Z_to_u64 annot_e]; rewrite ?insert_anon.
+Ltac type_step :=
   match goal with
+  | [ |- expr_hasTy _ _ _ ] => solve [eauto with types]
   | [ |- expr_hasTy _ _ _ ] => econstructor
+  | [ |- expr_hasTy _ (Rec _ (annot_e (annot _ ?t)) _) (arrowT _ _) ] => eapply (rec_expr_hasTy_eq t)
   | [ |- expr_hasTy _ (Rec _ _ _) (arrowT _ _) ] => eapply rec_expr_hasTy_eq
-  | [ |- val_hasTy _ _ _ ] => econstructor
-  | [ |- base_lit_hasTy _ _ ] => econstructor
+  | [ |- val_hasTy _ _ _ ] => solve [eauto with types] || econstructor
+  | [ |- base_lit_hasTy _ _ ] => solve [eauto with types] || econstructor
   end; simp.
 
 Ltac typecheck :=
   repeat (type_step; try match goal with
                          | [ |- _ = _ ] => cbv; reflexivity
                          end).
-
-Module slice_types.
-Section go_lang.
-  Context {ext:ext_op}.
-
-  Opaque Z_to_byte.
-  Opaque Z_to_u64.
-
-  Open Scope heap_types.
-
-  Theorem NewByteSlice_t : ⊢ NewByteSlice : arrowT intT (sliceT byteT).
-  Proof.
-    typecheck.
-  Qed.
-
-  Theorem MemCpy_t t : ⊢ MemCpy :
-      (* refT t -> refT t -> intT -> unitT *)
-      arrowT (refT t)
-             (arrowT (refT t)
-                     (arrowT intT unitT)).
-  Proof.
-    typecheck.
-  Qed.
-End go_lang.
-End slice_types.
